small edits

lib/Lib.ByteSequence.fsti
@@ -7,18 +7,20 @@ open Lib.Sequence
 
 /// Definition of byte-based sequences
 
-inline_for_extraction
-type bytes = seq uint8
+unfold inline_for_extraction
+type bytes_l (l:secrecy_level) = seq (uint_t U8 l)
 
-inline_for_extraction
-type lbytes (len:size_nat) = lseq uint8 len
+unfold inline_for_extraction
+type lbytes_l (l:secrecy_level) (len:size_nat) = lseq (uint_t U8 l) len
 
-inline_for_extraction
-let to_lbytes (b:bytes{length b > 0 /\ length b < max_size_t}) : lbytes (length b) =
-  to_lseq #uint8 b
+unfold inline_for_extraction let bytes = bytes_l SEC
+unfold inline_for_extraction let lbytes (len:size_nat) = lbytes_l SEC len
+unfold inline_for_extraction let pub_bytes = bytes_l PUB
+unfold inline_for_extraction let pub_lbytes (len:size_nat) = lbytes_l PUB len
 
+(* FIXME: the following function is a declassification! *)
 inline_for_extraction
-val lbytes_eq:#len:size_nat -> lseq uint8 len -> lseq uint8 len -> bool
+val lbytes_eq:#l:secrecy_level -> #len:size_nat -> lbytes_l l len -> lbytes_l l len -> bool
 
 /// Constant for empty lbytes
 
@@ -35,50 +37,50 @@ val nat_from_intseq_le: #t:inttype -> #l:secrecy_level
   -> b:seq (uint_t t l) -> n:nat{n < pow2 (length b * bits t)}
 
 inline_for_extraction
-val nat_from_bytes_be: b:bytes -> n:nat{n < pow2 (length b * 8)}
+val nat_from_bytes_be: #l:secrecy_level -> b:bytes_l l -> n:nat{n < pow2 (length b * 8)}
 
 inline_for_extraction
-val nat_from_bytes_le: b:bytes -> n:nat{n < pow2 (length b * 8)}
+val nat_from_bytes_le: #l:secrecy_level -> b:bytes_l l -> n:nat{n < pow2 (length b * 8)}
 
 inline_for_extraction
-val nat_to_bytes_be: len:nat -> n:nat{n < pow2 (8 * len)}
-  -> b:bytes{length b == len /\ n == nat_from_intseq_be #U8 b}
+val nat_to_bytes_be: #l:secrecy_level -> len:nat -> n:nat{n < pow2 (8 * len)}
+  -> b:bytes_l l{length b == len /\ n == nat_from_intseq_be #U8 b}
 
 inline_for_extraction
-val nat_to_bytes_le: len:nat -> n:nat{n < pow2 (8 * len)}
-  -> b:bytes{length b == len /\ n == nat_from_intseq_le #U8 b}
+val nat_to_bytes_le: #l:secrecy_level -> len:nat -> n:nat{n < pow2 (8 * len)}
+  -> b:bytes_l l{length b == len /\ n == nat_from_intseq_le #U8 b}
 
 inline_for_extraction
-val uint_to_bytes_le: #t:inttype -> #l:secrecy_level -> uint_t t l -> lbytes (numbytes t)
+val uint_to_bytes_le: #t:inttype -> #l:secrecy_level -> uint_t t l -> lbytes_l l (numbytes t)
 
 val index_uint_to_bytes_le: #t:inttype -> #l:secrecy_level -> u:uint_t t l
   -> Lemma
-    (forall (i:nat{i < numbytes t}). index (uint_to_bytes_le u) i ==
-                              u8 (uint_v u / pow2 (op_Multiply 8 i) % pow2 8))
+    (forall (i:nat{i < numbytes t}). index (uint_to_bytes_le #t #l u) i ==
+                              uint #U8 #l (uint_v u / pow2 (op_Multiply 8 i) % pow2 8))
 
 inline_for_extraction
-val uint_to_bytes_be: #t:inttype -> #l:secrecy_level -> u:uint_t t l -> lbytes (numbytes t)
+val uint_to_bytes_be: #t:inttype -> #l:secrecy_level -> u:uint_t t l -> lbytes_l l (numbytes t)
 
 inline_for_extraction
 val uint_from_bytes_le: #t:inttype{~(t == U1)} -> #l:secrecy_level
-  -> b:lbytes (numbytes t) -> uint_t t l
+  -> b:lbytes_l l (numbytes t) -> uint_t t l
 
 inline_for_extraction
 val uint_from_bytes_be: #t:inttype{~(t == U1)} -> #l:secrecy_level
-  -> lbytes (numbytes t) -> uint_t t l
+  -> lbytes_l l (numbytes t) -> uint_t t l
 
 inline_for_extraction
 val uints_to_bytes_le: #t:inttype -> #l:secrecy_level -> #len:size_nat{len * numbytes t < pow2 32}
-  -> lseq (uint_t t l) len -> lbytes (len * numbytes t)
+  -> lseq (uint_t t l) len -> lbytes_l l (len * numbytes t)
 
 inline_for_extraction
 val uints_to_bytes_be: #t:inttype -> #l:secrecy_level -> #len:size_nat{len * numbytes t < pow2 32}
-  -> lseq (uint_t t l) len -> lbytes (len * numbytes t)
+  -> lseq (uint_t t l) len -> lbytes_l l (len * numbytes t)
 
 inline_for_extraction
 val uints_from_bytes_le: #t:inttype{~(t == U1)} -> #l:secrecy_level -> #len:size_nat{len * numbytes t < pow2 32}
-  -> lbytes (len * numbytes t) -> lseq (uint_t t l) len
+  -> lbytes_l l (len * numbytes t) -> lseq (uint_t t l) len
 
 inline_for_extraction
 val uints_from_bytes_be: #t:inttype{~(t == U1)} -> #l:secrecy_level -> #len:size_nat{len * numbytes t < pow2 32}
-  -> lbytes (len * numbytes t) -> lseq (uint_t t l) len
+  -> lbytes_l l (len * numbytes t) -> lseq (uint_t t l) len
