lib/fst/Lib.ByteBuffer.fst
@@ -17,6 +17,38 @@ friend Lib.IntTypes
 friend Lib.ByteSequence
 friend Lib.Buffer
 
+let uint_to_be #t #l u =
+  match t with
+  | U1 -> u
+  | U8 -> u
+  | U16 -> C.Endianness.htobe16 u
+  | U32 -> C.Endianness.htobe32 u
+  | U64 -> C.Endianness.htobe64 u
+
+
+let uint_to_le #t #l u =
+  match t with
+  | U1 -> u
+  | U8 -> u
+  | U16 -> C.Endianness.htole16 u
+  | U32 -> C.Endianness.htole32 u
+  | U64 -> C.Endianness.htole64 u
+
+let uint_from_be #t #l u =
+  match t with
+  | U1 -> u
+  | U8 -> u
+  | U16 -> C.Endianness.be16toh u
+  | U32 -> C.Endianness.be32toh u
+  | U64 -> C.Endianness.be64toh u
+
+let uint_from_le #t #l u =
+  match t with
+  | U1 -> u
+  | U8 -> u
+  | U16 -> C.Endianness.le16toh u
+  | U32 -> C.Endianness.le32toh u
+  | U64 -> C.Endianness.le64toh u
 
 #set-options "--z3rlimit 50 --max_fuel 1 --max_ifuel 0"
 
